CCsub_Lemmas.v
@@ -377,13 +377,19 @@ Lemma wf_typ_subst_tb : forall F Q E Ap Am Z P T,
   wf_typ E Ap Am P ->
   wf_typ E Am Ap P ->
   ok (map (subst_tb Z P) F ++ E) ->
-  wf_typ (map (subst_tb Z P) F ++ E) Ap Am (subst_tt Z P T)
+  wf_typ (map (subst_tb Z P) F ++ E)
+         (subst_atoms Z (cset_fvars (cv P)) Ap)
+         (subst_atoms Z (cset_fvars (cv P)) Am) 
+         (subst_tt Z P T)
 with wf_pretyp_subst_tb : forall F Q E Ap Am Z P T,
   wf_pretyp (F ++ [(Z, bind_sub Q)] ++ E) Ap Am T ->
   wf_typ E Ap Am P ->
   wf_typ E Am Ap P ->
   ok (map (subst_tb Z P) F ++ E) ->
-  wf_pretyp (map (subst_tb Z P) F ++ E) Ap Am (subst_tpt Z P T).
+  wf_pretyp (map (subst_tb Z P) F ++ E)
+    (subst_atoms Z (cset_fvars (cv P)) Ap)
+    (subst_atoms Z (cset_fvars (cv P)) Am)
+    (subst_tpt Z P T).
 Proof with simpl_env; eauto using wf_typ_weaken_head, type_from_wf_typ, wf_cset_subst_tb.
 ------
   intros *. intros HwfT HwfPp HwfPm Hok.
@@ -391,13 +397,16 @@ Proof with simpl_env; eauto using wf_typ_weaken_head, type_from_wf_typ, wf_cset_
   generalize dependent F.
   induction HwfT; intros F EQF Hok; subst; simpl subst_tt.
   - Case "wf_typ_var".
-    destruct (X == Z); subst...
+    destruct (X == Z); subst.
+    + eapply wf_typ_weaken_head with (Ap := Ap) (Am := Am)...
+      1, 2: admit.
     + SCase "X <> Z".
       unfold wf_typ_in in *.
       binds_cases H...
       apply (wf_typ_var (subst_tt Z P U))...
   - unfold wf_typ_in in *.
     econstructor...
+    apply wf_cset_subst_tb.
 ------
   intros *. intros HwfT HwfPp HwfPm Hok.
   remember (F ++ [(Z, bind_sub Q)] ++ E).
